Exisits Working

matchingBlood.dfy
@@ -1,78 +1,94 @@
+include "bloodRep.dfy"
+include "dateRep.dfy"
 import B = BloodRep
+  import D = DateRep
 datatype BloodType = A | B | AB | O // A = 0, B = 1, AB = 2, O = 3
 datatype BloodRecord = BloodRecord(bType: BloodType, location: string, donationDate: D.Date, expiryDate: D.Date, isOkay: bool)
 
 method matchingBlood(patientBloodType: BloodType, a:array<BloodRecord>) returns (compatibleBlood: bool)
-    ensures patientBloodType == O && !doesExist(O, a) ==> compatibleBlood == false
-    ensures patientBloodType == O && doesExist(O, a) ==> compatibleBlood == true
-    ensures patientBloodType == A && doesExist(A, a) ==> compatibleBlood == true
-    ensures patientBloodType == A && !doesExist(A, a) && doesExist(O, a) ==> compatibleBlood == true
-    ensures patientBloodType == A && !doesExist(A, a) && !doesExist(O, a) ==> compatibleBlood == false
-    ensures patientBloodType == B && doesExist(B, a) ==> compatibleBlood == true
-    ensures patientBloodType == B && !doesExist(B, a) && doesExist(O, a) ==> compatibleBlood == true
-    ensures patientBloodType == B && !doesExist(B, a) && !doesExist(O, a) ==> compatibleBlood == false
-    ensures patientBloodType == AB && doesExist(AB, a) ==> compatibleBlood == true
-    ensures patientBloodType == AB && !doesExist(AB, a) && 
-        doesExist(A, a) ==> compatibleBlood == true
-    ensures patientBloodType == AB && !doesExist(AB, a) && 
-        !doesExist(A, a) && doesExist(B, a) ==> compatibleBlood == true
-    ensures patientBloodType == AB && !doesExist(AB, a) && 
-        !doesExist(A, a) && !doesExist(B, a) && doesExist(O, a) ==> compatibleBlood == true
-    ensures patientBloodType == AB && !doesExist(AB) && 
-        !doesExist(A, a) && !doesExist(B, a) && !doesExist(O, a) ==> compatibleBlood == false
+    requires a != null && a.Length > 0
+    ensures patientBloodType == O && !doesExistPredicate(O, a) ==> compatibleBlood == false
+    ensures patientBloodType == O && doesExistPredicate(O, a) ==> compatibleBlood == true
+    ensures patientBloodType == A && doesExistPredicate(A, a) ==> compatibleBlood == true
+    ensures patientBloodType == A && !doesExistPredicate(A, a) && doesExistPredicate(O, a) ==> compatibleBlood == true
+    ensures patientBloodType == A && !doesExistPredicate(A, a) && !doesExistPredicate(O, a) ==> compatibleBlood == false
+    ensures patientBloodType == B && doesExistPredicate(B, a) ==> compatibleBlood == true
+    ensures patientBloodType == B && !doesExistPredicate(B, a) && doesExistPredicate(O, a) ==> compatibleBlood == true
+    ensures patientBloodType == B && !doesExistPredicate(B, a) && !doesExistPredicate(O, a) ==> compatibleBlood == false
+    ensures patientBloodType == AB && doesExistPredicate(AB, a) ==> compatibleBlood == true
+    ensures patientBloodType == AB && !doesExistPredicate(AB, a) && 
+        doesExistPredicate(A, a) ==> compatibleBlood == true
+    ensures patientBloodType == AB && !doesExistPredicate(AB, a) && 
+        !doesExistPredicate(A, a) && doesExistPredicate(B, a) ==> compatibleBlood == true
+    ensures patientBloodType == AB && !doesExistPredicate(AB, a) && 
+        !doesExistPredicate(A, a) && !doesExistPredicate(B, a) && doesExistPredicate(O, a) ==> compatibleBlood == true
+    ensures patientBloodType == AB && !doesExistPredicate(AB, a) && 
+        !doesExistPredicate(A, a) && !doesExistPredicate(B, a) && !doesExistPredicate(O, a) ==> compatibleBlood == false
 {
-    if (patientBloodType == O && !doesExist(O, a))
+    var validO := doesExist(O, a);
+    var validA := doesExist(A, a);
+    var validAB := doesExist(AB, a);
+    var validB := doesExist(B, a);
+    if (patientBloodType == O && !validO)
     {
             compatibleBlood := false;
     }
-    if (patientBloodType == O && doesExist(O, a))
+    if (patientBloodType == O && validO)
     {
         compatibleBlood := true;
     }
-    if (patientBloodType == A && doesExist(A, a))
+    if (patientBloodType == A && validA)
     {
         compatibleBlood := true;
     }
-    if (patientBloodType == A && !doesExist(A, a) && doesExist(O, a))
+    if (patientBloodType == A && !validA && validO)
     {
         compatibleBlood := true;
     }
-    if (patientBloodType == A && !doesExist(A, a) && !doesExist(O, a))
+    if (patientBloodType == A && !validA && !validO)
     {
         compatibleBlood := false;
     }
-    if (patientBloodType == B && doesExist(B, a))
+    if (patientBloodType == B && validB)
     {
         compatibleBlood := true;
     }
-    if (patientBloodType == B && !doesExist(B, a) && doesExist(O, a))
+    if (patientBloodType == B && !validB && validO)
     {
         compatibleBlood := true;
     }
-    if (patientBloodType == B && !doesExist(B, a) && !doesExist(O, a))
+    if (patientBloodType == B && !validB && !validO)
     {
         compatibleBlood := false;
     }
-    if (patientBloodType == AB && doesExist(AB, a))
+    if (patientBloodType == AB && validAB)
     {
         compatibleBlood := true;
     }
 }
 
-method doesExist(a:array<BloodRecord>, bType: BloodType) returns (Exists: bool)
-    requires a != null && a.Length > 0
-    ensures Exists == exists k :: 0 <= k < a.Length && a[k].bType == bType
+method doesExist(bType: BloodType, a:array<BloodRecord>) returns (Exists: bool)
+    requires a != null
+    ensures Exists == true ==> exists k :: 0 <= k < a.Length && a[k].bType == bType
 {
     var i := 0;
     Exists := false;
     while (i < a.Length)
         decreases a.Length - i
         invariant 0 <= i <= a.Length
-        invariant Exists == true ==> exists k :: 0 <= k <= i && a[k].bType == bType 
+        invariant Exists == true ==> exists k :: 0 <= k < i && a[k].bType == bType 
     {
         if (a[i].bType == bType)
         {
             Exists := true;
         }
+
+        i := i + 1;
     }
+}
+
+predicate doesExistPredicate(bType: BloodType, a:array<BloodRecord>)
+    reads a
+{
+    exists k :: 0 <= k < a.Length && a[k].bType == bType
 }
