bloodRep.dfy
@@ -1,4 +1,4 @@
-
+include "dateRep.dfy"
 module BloodRep {
   import D = DateRep
   datatype BloodType = A | B | AB | O // A = 0, B = 1, AB = 2, O = 3
